\section{Asymptotics of $\Tr{(\Delta_\lambda + z^2)^{-2}}$}

\section{Compilation}
Now that we have calculated the coefficients we only need to integrate the
homogeneous part with the logarithm. To do that we use the Mellin transform,
since
\begin{align*}
    \left.\frac\partial{\partial z} \Integ[\infty]{0}{x}{x^z f(x)}\right|_{z=0}
    &= \Integ[\infty]{0}{x}{\ln{(x)} f(x)}
\end{align*}
if one of the integrals exist. We thus calculate:
\begin{align*}
    \Integ[\infty]{0}{\lambda}{\frac{\lambda^{n + z}}{\left(1 +
    \lambda^2\right)^{\frac{n+5}{2}}}} &=
    % Substituiere \lambda^2 = y
    \frac12\Integ[\infty]{0}{y}{\frac{y^{\frac{n+z+1}{2}}}{(1 +
    y)^{\frac{n+5}{2}}}} \\
    % Betafunktion
    &= \frac12 B\left(\tfrac{n+z+1}{2}, \tfrac{4-z}{2}\right)
\end{align*}
where $B(a,b)$ is the beta function. % Benutztes Integral mit ref!
% a = n+z+1/2, b = n+5/2 - a
% Eigenschaften, insbesondere B(a,b) = Gamma(a)Gamma(b) / Gamma(a+b)

The function is symmetric, and its
derivative is $\partial_a B(a,b) = B(a,b) (\psi(a) - \psi(a+b))$, where
$\psi(x) = \partial_x \ln\Gamma(x)$ is the digamma function, so we get
\begin{align*}
    \left.\frac12\frac\partial{\partial z} B\left(\tfrac{n+z+1}{2}, \tfrac{4-z}{2}\right)\right|_{z=0}
    &= \left.\frac14 B\left(\tfrac{n+z+1}{2}, \tfrac{4-z}{2}\right)
    \left(\psi\left(\tfrac{n+z+1}{2}\right) - \psi\left(\tfrac{n+5}{2}\right) -
    \psi\left(\tfrac{4-z}{2}\right) +
    \psi\left(\tfrac{n+5}{2}\right)\right)\right|_{z=0} \\
    &= \frac14 B\left(\tfrac{n+1}{2}, 2\right)
    \left(\psi\left(\tfrac{n+1}{2}\right) - \psi\left(2\right)\right)
\end{align*}

$B(\tfrac{n+1}{2}, 2)$ can be evaluated using the formula given above to be
$\tfrac{4}{(n+1)(n+3)}$. Using the recurrence relation $\psi(x + 1) = \psi(x) +
\frac{1}{x}$ and the special values $\psi(1) = -\gamma$ and $\psi(\tfrac{1}{2})
= -\gamma - 2\ln 2$ ($\gamma$ being the Euler-Mascheroni constant) we arrive at
the following explicit formula for the integral:
\begin{align*}
    \Integ[\infty]{0}{\lambda}{\frac{\lambda^n}{(1 +
    \lambda^2)^{\frac{n+5}{2}}}\ln{\lambda}} = \frac{1}{(n+1)(n+3)}
        \begin{cases} 
            -1 - 2\ln 2 + \sum_{k=1}^{\frac n 2}\frac{2}{2k - 1} & n\text{
            even} \\
            -1 + \sum_{k=1}^{\frac{n-1}{2}}\frac 1 k & n\text{ odd}
        \end{cases}
\end{align*}
