\section{Asymptotics of the exterior parametrix}
By using the summation formula derived in LV12 the existence and values of the
asymptotic components of the specific operator we're looking at can be
calculated directly. From Lemma bla we know, that we only have to consider $j\in
{0, 1, 2}$ since the requested asymptotic coefficient is of order $-5$ % TODO

The calculation for $j=0$ is straightforward:
\begin{align}
    \Tr R^{(0)} =& \Integ[1]{0}{x}{k_\theta(x,x;\mu) - k_\mathbb{R}(x,x;\mu)} \\
    =& -\frac1{2\mu} C(\mu,\theta) \Integ[1]{0}{x}{\Eto{-2\mu x}} \\
%    =& -\frac1{2\mu} C(\mu,\theta) \left( \frac1{2\mu} - \frac{\Eto{-2\mu}}{2\mu} \right) \\
    \SimAs{\mu\to\infty}& -\frac1{4\mu^2}
    \label{eqn:jeq0}
\end{align}

For $j=1$ and $j=2$ we employ the following Lemma:
\begin{Lemma}[Watson]
    \input{snippets/watsons-lemma}
    \begin{proof}
        See Appendix~\ref{sec:proof-watson}.
    \end{proof}
    \begin{Remark}
        We actually don't need analyticity but only the existence of as many
        derivatives as degrees we want and additionally a finiteness condition
        on
    \end{Remark}
\end{Lemma}

% j = 1, ++
% TODO: 1/2Âµ einbauen
The first term for $j=1$ is as follows
\begin{align*}
    \Tr R^{(1)}_{++} &= C(\mu,\theta)^2
        \Integ[1]{0}{x}{
            \Integ[1]{0}{z}{\Eto{-\mu(x+z)}
                \lambda(z)\Eto{-\mu(z+x)}
            }
        }
        \\
        &= C(\mu,\theta)^2
            \Integ[1]{0}{x}{
                \Eto{-2\mu x}
            }
            \Integ[1]{0}{z}{\Eto{-2\mu z}\lambda(z)}
        \\
        &= C(\mu, \theta)^2 \left(
            \frac1{2\mu} - \frac{\Eto{-2\mu}}{2\mu}
           \right)
           \Integ[1]{0}{z}{\Eto{-2\mu z}\lambda(z)}
        \\
        &\SimAs{\mu\to\infty}
            \frac{(-1)^2}{2\mu}
            \sum_{n=0}^{\infty}\frac{\lambda^{(n)}(0)}{(2\mu)^{n+1}}
\end{align*}

% j = 1, +-
The second term for $j=1$ is
\begin{align*}
    \Tr R^{(1)}_{+-} &= -C(\mu,\theta)
        \Integ[1]{0}{x}{
            \Integ[1]{0}{z}{\Eto{-\mu(x+z)}
                \lambda(z)\Eto{-\mu\left|z-x\right|}
            }
        } \\
        &= -C(\mu,\theta)
            \Integ[1]{0}{x}{\left(
                \Integ[x]{0}{z}{
                    \Eto{-\mu(x+z+x-z)} \lambda(z)
                }
                +
                \Integ[1]{x}{z}{
                    \Eto{-\mu(x+z-x+z)} \lambda(z)
                }
                \right)
            } \\
        &= -C(\mu,\theta) \left(
            \Integ[1]{0}{x}{\Eto{-2\mu x} \Lambda(x)}
            + \Integ[1]{0}{x}{\Eto{-2\mu x}\lambda(x)x}
            \right) \\
        &\SimAs{\mu\to\infty}\ 
            \sum_{n=0}^\infty \frac{\Lambda^{(n)}(0)}{(2\mu)^{n+1}}
            + \sum_{n=0}^\infty \frac{n\lambda^{(n-1)}(0)}{(2\mu)^{n+1}} \\
        &= \sum_{n=0}^\infty \frac{(n+1)\lambda^{(n-1)}}{(2\mu)^{n+1}}
\end{align*}
% TODO: Beweis, dass Int_0^1 Int_y^1 f(x) dx dy = Int_0^1 x f(x) dx
% TODO: (x*f(x))^(n) = x*f^(n) + n*f^(n-1)
where $\Lambda(x) := \Integ[x]{0}{z}{\lambda(z)}$.
