\section{Setting}
We will first motivate our investigation of the asymptotics of multi-parametric
Sturm-Liouville operators by a formula given in \cite{LV13}. This formula can be
used to calculate the zeta determinant of an infinite direct sum of
Sturm-Liouville operators by means of a regularised sum of the zeta determinants
of the operators and an error term involving a specific (poly-)homogeneous
component of the asymptotic expansion of the direct sum operator.

We will first introduce the toy example of a surface of revolution, which indeed
decomposes into an infinite sum of Sturm-Liouville operators, and then introduce
the further notation needed to understand the formula, whose error term we aim
to calculate in the end.

\subsection{Laplace-Beltrami operator on a surface of revolution}
\label{sec:laplace-beltrami}
Let $M = [0,1]\times\Sphere{1}$ be a surface of revolution by use of the metric
$g = \mathrm dx^2 \oplus f(x)^2 g_\Sphere{1}$ with $f\in \Cinf([0,1],
\Rplus)$. The associated Laplace-Beltrami operator is given by
\begin{align}
  \Delta = -\frac{\partial^2}{\partial x^2} -
            \frac{f'(x)}{f(x)}\frac{\partial}{\partial x} +
            \frac{1}{f(x)^2}\Delta_\Sphere1,
  \label{eqn:laplace}
\end{align}
acting on $\Cinf[0]\bigl((0,1)\times\Sphere1\bigr)$. The correct Lebesgue
measure on the space $(M,g)$ is given by $f(x)\,\mathrm dx\, \mathrm
d\!\vol(g_\Sphere1)$. Under the unitary map
\begin{align*}
  \Phi\colon L^2(M, g)&\to L^2([0,1], \mathrm dx)\otimes L^2(\Sphere1,
  g_\Sphere1) \\ (\Phi u)(x) &:= u(x) \sqrt{f(x)},
\end{align*}
the Laplacian $\Delta$ transforms into the operator
\begin{align*}
  \Phi\Delta\Phi^{-1} = -\frac{\partial^2}{\partial x^2} +
  \frac{1}{f(x)^2}\Delta_\Sphere1 + \left( \frac{f''(x)}{2f(x)} -
  \left(\frac{f'(x)}{2f(x)}\right)^2\right).
\end{align*}
For $\lambda\in\mathbb{Z}$ the functions $e_\lambda(x) :=
\frac{1}{\sqrt{2\pi}}\Eto{\mathrm i\lambda x}$ form an orthonormal basis of
$L^2(\Sphere1)$ of eigenfunctions of $\Delta_\Sphere1$ to the eigenvalues
$\lambda^2$, where the eigenvalues $\lambda^2 \neq 0$ have multiplicity 2 while
$\lambda = 0$ has multiplicity 1. Hence we have the decomposition
\begin{align}
  \label{eqn:lpl-decomp}
  \Phi\Delta\Phi^{-1} &= \bigoplus_{\lambda=-\infty}^{\infty} \left(
    -\frac{\partial^2}{\partial x^2} + \frac{\lambda^2}{f(x)^2} + 
     \left( \frac{f''(x)}{2f(x)} -
     \left(\frac{f'(x)}{2f(x)}\right)^2\right)\right)
     =: \bigoplus_{\lambda=0}^{\infty}\Delta_\lambda
\end{align}
into a direct sum of one-dimensional Sturm-Liouville operators $\Delta_\lambda$.
We consider separated Dirichlet or generalised Neumann boundary conditions for
$\Delta$, where it is straight-forward to see, that those also correspond to
separated Dirichlet, resp.\ generalised Neumann boundary conditions for
$\Phi\Delta\Phi^{-1}$ and that the resulting self-adjoint operator is compatible
with the given decomposition \eqref{eqn:lpl-decomp}. Since the transformed
operator does indeed behave, from an analytical point of view, the same as the
operator $\Delta$ we will denote the self-adjoint extensions of $\Delta$ and
$\Delta_\lambda$ again by the same name. Since we are considering fixed boundary
conditions this is not too ambiguous.

We will consider operators like $\Delta_\lambda$, where we will set
\begin{align}
  V(x) &:= f(x)^{-2} \\
  W(x) &:= \frac{f''(x)}{2f(x)} - \left(\frac{f'(x)}{2f(x)}\right)^2 =
  \partial_x^2 \log\sqrt{f(x)} + \left(\partial_x \log\sqrt{f(x)}\right)^2 \\
  \text{thus}\quad \Delta_\lambda &= -\partial^2_x + \lambda^2 V(x) + W(x),
\end{align}
where the non-derivative terms as usual denote the multiplication operators
$(M_\phi u)\colon x \mapsto \phi(x)u(x)$. We won't write this out, i.e.\ in the
summands of $\Delta_\lambda$ we use $W(x)$ instead of $M_W$.

In our calculations we will not depend on the specific choice of $V$ and $W$,
but instead only require
\begin{align*}
  &V,W\in\Cinf([0,1]) \\
  &\forall_{x\in[0,1]}\colon V(x) > 0 \\
  &V\text{ and }W\text{ analytic in neighbourhoods of $0$ and $1$}.
\end{align*}
If $f$ is analytic and $f>0$ this is given.

\subsection{Regularised Sums and Integrals}
\label{sec:regsum-int}
We will first provide some general definitions on asymptotic analysis based on
\cite[Ch.1]{Miller2006} and then introduce the Hadamard finite part regularisation.
\begin{Definition}
  The Landau symbols and asympotic equality are defined as
  \begin{align}
    g(x) = O(f(x))\text{ for $x\to x_0$ } &:\Leftrightarrow \limsup_{x\to x_0}
    \Abs{\frac{g(x)}{f(x)}} < \infty \\
    g(x) = o(f(x))\text{ for $x\to x_0$ } &:\Leftrightarrow \lim_{x\to
    x_0}\Abs{\frac{g(x)}{f(x)}} = 0 \\
    f \SimAs{x\to x_0} g &:\Leftrightarrow \lim_{x\to x_0}
    \Abs{\frac{f(x)}{g(x)}} = 1,
  \end{align}
  where $x_0$ may be $\infty$. As a special case we furthermore define for
  $x\to\infty$
  \begin{align}
    f(x) = O(x^{-\infty}) :\Leftrightarrow \forall_{n\in\mathbb{N}}\ f(x) =
    O(x^{-n}).
  \end{align}
\end{Definition}
Like in many other texts we will also use the Landau symbols in actual
calculations, however it is of note, that this is only valid in finite sums, for
all other calculations (in particular integrations) we have to take additional
measures.

\begin{Definition}
  Let $(\phi_n)$ be a sequence of functions with
\begin{align*}
  \phi_{n+1}(x) = o(\phi_n(x))\text{ for $x\to x_0$},
\end{align*}
  which is called an \emph{asymptotic sequence}. Then, for a sequence $(a_n)$
  the sum
  \begin{align*}
    \sum_{n=0}^N a_n\phi_n(x)
  \end{align*}
  is an \emph{asymptotic approximation} as $x\to x_0$ if
  \begin{align*}
    \label{eqn:def-asymp-exp}
    f(z) - \sum_{n=0}^N a_n\phi_n(x) = o(\phi_N(x)).
  \end{align*}
  If the above is true for all $N\in\mathbb{N}$, the formal infinite sum
  \begin{align*}
    \sum_{n=0}^\infty a_n\phi_n(x)
  \end{align*}
  is called an \emph{asymptotic series} and is said to be an \emph{asymptotic
  expansion} of $f(x)$, which we will denote by
  \begin{align*}
    f(x) \SimAs{x\to x_0} \sum_{n=0}^\infty a_n\phi_n(x).
  \end{align*}.
  If \eqref{eqn:def-asymp-exp} holds for all $N < N_0$, we say $f(x)$ has a
  \emph{partial asymptotic expansion}.
\end{Definition}
Now let $f\in\Cinf(\Rplus)$ be a function with a partial asymptotic expansion
for $x\to\infty$ with regard to the log-polynomial asymptotic series
$x^{-n}\log^k(x)$, were $\log^k(x) := (\log(x))^k$. We denote the components by
$a_{nk}$, thus the expansion is written as
\begin{align*}
  f(x) \SimAs{x\to\infty} \sum_{n=0}^{N-1}\sum_{k=0}^{M_n}
  a_{nk}\,x^{-n}\log^k(x) + x^{-N}\log^{M_N}f_N(x),
\end{align*}
where $N\in\mathbb{N}$ is arbitrary and the remainder is $f_N(x) = o(1)$ as
$x\to\infty$. We define the \emph{regularised limit} for $x\to\infty$ as
\begin{align}
  \Reglim_{x\to\infty} f(x) := a_{00},
\end{align}
i.e.\ as the constant part of the expansion.

If for some $N\in\mathbb{N}$ the remainder $(x\mapsto x^{-N}f_N(x))\in
L^1[1,\infty)$, the integral $\Integ[R]{1}{x}{f(x)}$ does also admit an
asymptotic expansion of the form given above and we define its \emph{regularised
integral} as
\begin{align}
  \Regint{x}{f(x)} := \Reglim_{R\to\infty}\Integ[R]{1}{x}{f(x)}.
\end{align}
The integral is also the reason why we consider $x^n \log^m(x)$ as
base-functions in the asymptotic expansions, since that way the integral over
the expansion results in a meaningful expansion with the same base-functions.
This approach of regularising potentially infinite integrals is called Hadamard
finite part (or French: \textit{partie finie}) regularisation. In the special
case that $f\in L^1[1,\infty)$ the regularised integral coincides with the usual
Lebesgue integral of $f$.

Using this we can also give a meaningful definition of a \emph{regularised sum}
over $f$. Given the Bernoulli numbers $B_j$ and the Bernoulli polynomials
$B_j(x)$ consider the Euler-MacLaurin summation formula:
\begin{align*}
  \sum_{\lambda=1}^N f(\lambda) &= \Integ[N]{1}{x}{f(x)}
  + \sum_{k=1}^M \frac{B_{2k}}{(2k)!}\left(f^{(2k-1)}(N) - f^{(2k-1)}(1)\right)
  \\
  &\mathbin{+} \frac1{(2M + 1)!}\Integ[N]{1}{x}{B_{2m+1}(x-[x])f^{(2M+1)}(x)}
  \\
  &\mathbin{+} \frac12(f(1)+f(N))
\end{align*}
By essentially replacing the integrals by regularised integrals we arrive at the
following definition for the regularised sum:
\begin{align*}
  \Regsum_{\lambda=1}^\infty f(\lambda) := \Reglim_{N\to\infty} \sum_{\lambda=1}^N
  f(\lambda)
\end{align*}
The regularised sum over $\mathbb{Z}$ is defined by
\begin{align*}
  \Regsum_{\lambda\in\mathbb{Z}} f(\lambda) := f(0) + \Regsum_{\lambda=1}^\infty
  f(\lambda) + \Regsum_{\lambda=1}^\infty f(-\lambda)
\end{align*}

The following theorem proven in \cite{LV13} is the basis for the following
considerations:
\begin{Theorem}
  \label{thm:fubini}
  Assume $f\in\Cinf(\Rplus[2])$ is of the form
  \begin{align*}
    f(x,y) = \sum_{j=0}^{N-1} f_{\alpha_j}(x,y) + F_N(x,y)
  \end{align*}
  where $N\in\mathbb{N}$ and each $f_{\alpha_j}\in\Cinf(\mathbb{R}_+^2\setminus\{0\})$
  is homogeneous of order $\alpha_j\in\mathbb{C}$ in both variables jointly,
  where the remainder $F_N$ is assumed to be in $L^1[1,\infty)^2$. Then
  \begin{align}
    \Regint{x}{\Regint{y}{f(x,y)}} =
    \Regint{y}{\Regint{x}{f(x,y)}} + \Integ[\infty]{0}{y}{f_{-2}(1,y)\log(y)}.
  \end{align}
\end{Theorem}
Using this Fubini-like theorem we can (possibly) simplify difficult regularised
integral, however unlike for Fubini's theorem in usual integral theory we get an
additional error term as an integral over one homogeneous component. 

\subsection{Zeta Determinants}
The zeta-function of an operator $\Delta_\lambda$ is defined for $\Re(s) > 0$
sufficiently large by
\begin{align}
  \zeta(s,\Delta_\lambda) :=
  \sum_{\mu\in\operatorname{spec}\Delta_\lambda\setminus\{0\}} m(\mu)\mu^{-s},
\end{align}
where $m(\mu)$ is the multiplicity of the eigenvalue $\mu > 0$. Using the
identity
\begin{align}
  \label{frm:zeta-frm}
  \zeta(s,\Delta_s) = 2 \frac{\sin\pi
  s}{\pi}\Regint[0]{z}{z^{1-2s}\Tr(\Delta_\lambda + z^2)^{-1}}
\end{align}
one can derive a formula for $\log\zdet\Delta_\lambda =
-\zeta'(0,\Delta_\lambda)$ (which is defined by the meromorphic extension to
$\mathbb{C}$ of $\zeta$) for which $s=0$ is a regular point:
\begin{align}
  \log\zdet\Delta_\lambda = -2\Regint[0]{z}{z\Tr(\Delta_\lambda + z^2)^{-1}}
\end{align}
However the resolvent $(\Delta + z^2)^{-1}$ is not trace class, $\zdet\Delta$
can not be defined in the exact same way. Integrating
Formula~\eqref{frm:zeta-frm} by parts we get
\begin{align}
  \zeta(s,\Delta_\lambda) = 2\frac{\sin\pi
  s}{\pi(1-s)}\Regint[0]{z}{z^{3-2s}\Tr(\Delta_\lambda + z^2)^{-2}},
\end{align}
and thus
\begin{align}
  \log\zdet\Delta_\lambda = -2 \Regint[0]{z}{z^3\Tr(\Delta_\lambda + z^2)^{-2}},
\end{align}
which also works for $\Delta$, since we have an asymptotic expansion for
$\Tr(\Delta_\lambda + z^2)^{-2}$.

\subsection{Goal}
Lesch and Vertman proved in \cite{LV13} the following asymptotic expansion for
the squared resolvent-trace of the operator given in \eqref{eqn:laplace}:
\begin{align}
  \Tr(\Delta + z^2)^{-2} = \sum_{\lambda=-\infty}^\infty \Tr(\Delta_\lambda +
  z^2)^{-2} \SimAs{z\to\infty} \sum_{k=2}^{\infty} a_kz^{-k}.
\end{align}
Using this asymptotic expansion and \thref{thm:fubini} they showed, that the
zeta-determinant of $\Delta$ is given by a regularised sum of the
zeta-determinants of the $\Delta_\lambda$ with an error term:
\begin{align}
  \label{eqn:central-thm}
  \log\zdet\Delta = \Regsum_{\lambda=-\infty}^\infty
  \log\zdet\Delta_\lambda -
  4\Integ[\infty]{0}{\lambda}{h_2(\lambda, 1)\log(\lambda)},
\end{align}
where $h_2(\lambda, z)$ denotes the homogeneous term of degree $-5$ (i.e.\ the
second non-vanishing term) in the polyhomogeneous asymptotic expansion of
$\Tr(\Delta_\lambda + z^2)^{-2}$ as $\Abs{(\lambda, z)}\to\infty$. The ultimate
goal of this thesis is to calculate the error term by calculating the first few
terms in the polyhomogeneous trace-expansion of the resolvent of a
Sturm-Liouville operator, since by formally deriving $\Tr(\Delta_\lambda +
z^2)^{-1}$ we see that
\begin{align}
  \label{frm:shift}
  \partial_z \Tr{(\Delta_\lambda + z^2)}^{-1} &=
        (-2z) \Tr{(\Delta_\lambda + z^2)}^{-2} \\
        \Leftrightarrow \Tr(\Delta_\lambda + z^2)^{-2} &=
        (-2z)^{-1}\partial_z\Tr(\Delta_\lambda + z^2)^{-1},
\end{align}
thus the order of the homogeneous components is from the resolvent to the
squared resolvent is shifted by 2. This means, that to get the component of
order $-5$ we will need to find the homogeneous component in the trace-expansion
of the parametrix of order $-3$.
