\section{Calculation of the next homogeneous component at the boundary}

% TODO: Auswalzen warum Stetigkeit ausreicht.

% j = 2
The calculations for $j = 2$ are a bit more involved. We start off with the case
$\Tr R^{(2)}_{++-} =  \Tr R^{(2)}_{-++}$:
% -++
\begin{align*}
  \Tr R^{(2)}_{-++} &= C_{-++} \Int{x}{
  \Int{z_1}{
    \Int{z_2}{
      \Eto{-\mu(\Abs{x-z_1} + z_1 + z_2 + z_2 + x)}
      \lambda(z_1)\lambda(z_2)
    }
  }
  } \\
  &= C_{-++} \Int{z_2}{\Eto{-2\mu z_2}\lambda(z_2)}
  \Int{x}{
    \left(
    \Integ[x]{0}{z_1}{
      \Eto{-2\mu x}\lambda(z_1)
    }
    + \Integ[1]{x}{z_1}{
      \Eto{-2\mu z_1}\lambda(z_1)
    }
    \right)
  } \\
  &= C_{-++} \Int{z}{\Eto{-2\mu z}\lambda(z)}
  \Int{x}{\Eto{-2\mu x}(\Lambda(x) + x\lambda(x))} \\
  &\SimMu (2\mu)^{-4} \Wsum{\lambda^{(n)}} \Wsum[1]{(n+1)\lambda^{(n-1)}}.
\end{align*}
Very similar to that we can calculate $\Tr R_{+-+}$:
% +-+
\begin{align*}
  \Tr R_{+-+}^{(2)} &= C_{+-+} \Int{x}{
    \Int{z_1}{
      \Int{z_2}{
        \Eto{-\mu(x+z_1 + \Abs{z_1 - z_2} + z_2 + x)}
        \lambda(z_1)\lambda(z_2)
      }
    }
  } \\
  &= C_{+-+} \Int{x}{\Eto{-2\mu x}}
  \Int{z_1}{
    \left(
    \Integ[1]{z_1}{z_2}{
      \Eto{-2\mu z_2}\lambda(z_1)\lambda(z_2)
    }
    + \Integ[z_1]{0}{z_2}{
      \Eto{-2\mu z_1}\lambda(z_1)\lambda(z_2)
    }
    \right)
  } \\
  &= C_{+-+} \Int{x}{\Eto{-2\mu x}}
    \Int{z}{
      \Eto{-2\mu z}\left(
        \Lambda(z)\lambda(z) + z (\lambda(z))^2
      \right)
    } \\
  % Result
    &\SimMu (2\mu)^{-5} \sum_{n=0}^\infty \frac{(\Lambda\lambda)^{(n)} +
  (z(\lambda(z))^2)^{(n)}(0)}{(2\mu)^{n+1}}
\end{align*}

% --+
Finally we arrive at the two most difficult terms, involving two absolute values
in the exponent, first $\Tr R_{--+}^{(2)}$:
\begin{align*}
  \Tr R_{--+}^{(2)} &= C_{--+} \Int{x}{
    \Int{z_1}{
      \Int{z_2}{
        \Eto{-\mu(\Abs{x-z_1} + \Abs{z_1 - z_2} + z_2 + x)}
        \lambda(z_1)\lambda(z_2)
      }
    }
  } \\
  = C_{--+} \Int{x}{\Bigl( \\
    % (I) x < z_1 < z_2
    &\Integ[1]{x}{z_1}{\Integ[1]{z_1}{z_2}{
        \Eto{-2\mu z_2}\lambda(z_1)\lambda(z_2)
      }
    } \\ &+
    % (III) x < z_1, z_2 < z_1 
    \Integ[1]{x}{z_1}{\Integ[0]{z_1}{z_2}{
        \Eto{-2\mu z_1}\lambda(z_1)\lambda(z_2)
      }
    } \\ &+
    % (IV) x < z_2 < z_1
    \Integ[x]{0}{z_1}{\Integ[z_1]{0}{z_2}{
        \Eto{-2\mu x}\lambda(z_1)\lambda(z_2)
      }
    } \\ &+
    % (II) x > z_1, x > z_2
      \Integ[x]{0}{z_1}{\Integ[1]{z_1}{z_2}{
        \Eto{-2\mu (x + z_2 - z_1)}\lambda(z_1)\lambda(z_2)
      }
    }
    \Bigr)
  }
\end{align*}
After splitting the Integral in those four terms we evaluate them one by one:
\begin{enumerate}[(I)]
  \item Using $\Integ[x]{0}{z}{z\lambda(z)} = x\Lambda(x) - M(x)$ we have:
    \begin{align*}
      \Int{x}{
        \Integ[1]{x}{z_1}{\Integ[1]{z_1}{z_2}{
            \Eto{-2\mu z_2}\lambda(z_1)\lambda(z_2)
          }
        }
      }
      &= \Int{z_1}{z_1 \Integ[1]{z_1}{z_2}{\Eto{-2\mu z_2}\lambda(z_1)\lambda(z_2)}}
      \\
      &= \Int{z_2}{\Eto{-2\mu z_2}\lambda(z_2) \Integ[z_2]{0}{z_1}{z_1\lambda(z_1)}}
      \\
      &\SimMu \Wsum{(x\lambda\Lambda - \lambda M)^{(n)}}
    \end{align*}

  \item
    \begin{align*}
      \Int{x}{
        \Integ[1]{x}{z_1}{
          \Integ[z_1]{0}{z_2}{
            \Eto{-2\mu z_1}{\lambda(z_1)\lambda(z_2)}
          }
        }
      }
      &= \Int{z_1}{z_1 \Eto{-2\mu z_1}\lambda(z_1)\Lambda(z_1)} \\
      &\SimMu \Wsum{(z\lambda\Lambda)^{(n)}}
    \end{align*}

  \item
    \begin{align*}
      \Int{x}{
        \Integ[x]{0}{z_1}{
          \Integ[z_1]{0}{z_2}{
            \Eto{-2\mu x}\lambda(z_1)\lambda(z_2)
          }
        }
      }
      &= \Int{x}{
        \Eto{-2\mu x} \Integ[x]{0}{z_1}{\lambda(z_1)\Lambda(z_1)}
      } \\
      &\SimMu \sum_{n=1}^\infty \frac{(\lambda\Lambda)^{(n-1)}}{(2\mu)^{n+1}}
    \end{align*}

  \item After those pretty straight-forward calculations we are left with a more
    difficult one:
    \begin{align*}
      \Int{x}{
        \Eto{-2\mu x}
        &\Integ[x]{0}{z_1}{
          \Eto{+2\mu z_1} \lambda(z_1)
          \Integ[1]{z_1}{z_2}{
            \Eto{-2\mu z_2} \lambda(z_2)
          }
        }
      } \\
      =&\Int{z_1}{
        \Eto{2\mu z_1}\lambda(z_1)
        \Integ[1]{z_1}{z_2}{
          \Eto{-2\mu z_2}\lambda(z_2)
        }
        \frac{1}{2\mu}\left(\Eto{-2\mu z_1} - \Eto{-2\mu}\right)
      } \\
      =&\ \frac{1}{2\mu}
        \Int{z_1}{
          \lambda(z_1)
          \Integ[1]{z_1}{z_2}{
            \Eto{-2\mu z_2}\lambda(z_2)
          }
        }
        -\frac{1}{4\mu}
        \left(\Int{z}{\Eto{-2\mu z}\lambda(z)}\right)^{2}
        \\
        =&\ \frac{1}{2\mu} \Int{z_2}{\Eto{-2\mu z_2}\lambda(z_2)\Lambda(z_2)}
        -\frac1{4\mu}\left(\Int{z}{\Eto{-2\mu z}\lambda(z)}\right)^{2}
        \\
        &\ \SimMu \sum_{n=1}\frac{(\lambda \Lambda)^{(n-1)}}{(2\mu)^{n+1}}
              -\frac{1}{4\mu}\left(\Wsum{\lambda^{(n)}}\right)^2
    \end{align*}
    % TODO Finalize
\end{enumerate}
which leads us to
\begin{align*}
  \Tr R_{--+}^{(2)}
  &= (2\mu)^{-4} \sum_{n=1}^{\infty}
  \frac{
    (M + 2x\lambda\Lambda)^{(n)}(0)
    + 2(\lambda\Lambda)^{(n-1)}(0)
  }{(2\mu)^n}
\end{align*}

% -+-
\begin{align*}
  \Tr R_{-+-}^{(2)} &= C_{-+-} \Int{x}{
    \Int{z_2}{
      \Int{z_1}{
        \Eto{-\mu(\Abs{x-z_1}+z_1+z_2+\Abs{z_2-x})}\lambda(z_1)\lambda(z_2)
      }
    }
  } \\
  &= C_{-+-} \Int{x}{
    \Eto{-2\mu x}
    \left(
      \Lambda(x)^2 + 2\lambda(x)M(x)
      % TODO: Dritter Term ist noch nicht 
      % gerechnet!
    \right)
  }
\end{align*}
